all lemmas are in the lemma file

Isabelle/Simdpll.thy
@@ -1,20 +1,17 @@
 theory Simdpll 
-imports Main
+imports Main 
 
 begin
 datatype 'a Option      =  None | Some 'a
 type_synonym    Literal =  int  
 type_synonym  Clause    =  "Literal list" 
 type_synonym Formula    =  "Clause list"
-type_synonym Model      =  "Literal set"
+type_synonym Model      =  "int list"
 
 fun negateLiteral :: "(Literal) \<Rightarrow>  Literal "
 where
 "negateLiteral  a =   (-1*a)"
 
-value "negateLiteral 1" 
-value "negateLiteral 0"
-value "negateLiteral (-1::int)"
 
 fun deOption::"(Formula) Option \<Rightarrow> Formula"
 where
@@ -28,10 +25,6 @@ where
 |
 "findUnit (c#cs) = (if length c = 1 then Some (hd c) else findUnit cs)"
 
-value "findUnit [[1,2,3],[1],[2]]" 
-value "findUnit [[],[1,2],[2]]"
-value "findUnit [[1,2]]"
-
 
 fun notElem :: "(Literal) \<Rightarrow> Clause \<Rightarrow> bool" 
 where
@@ -39,9 +32,6 @@ where
 |
 "notElem p (x#xs) = (if p=x then False else notElem p xs)"
 
-value "notElem 1 [1,2,3]"
-value "notElem 4 [1,2,3]"
-value "notElem 1 [] "
 
 fun elem :: "Clause \<Rightarrow> Formula \<Rightarrow>bool"
 where
@@ -50,47 +40,18 @@ where
 "elem p (x#xs) = (if p=x then True else elem p xs)"
 
 
-value "elem [] [[]]"
 (*should work on termination of this function *)
 fun resolve ::"Formula \<Rightarrow> Literal \<Rightarrow> Formula"
 where
 "resolve f literal =  (let  q = filter (notElem literal) f in map (removeAll (negateLiteral literal)) q)"
 
-value "resolve [[-1]] (-1::int)"
-value "resolve [[1,2,3],[-1,2,3],[4]] 1"
-
-lemma 1[simp]: "resolve [] a = []"
-apply simp
-done
 
 
-(*the other proof for the lemma which help the simp for unitpropagate termination*)
-lemma yes: "findUnit f = Some x \<Longrightarrow> length (filter (notElem x) f) < length f"
-proof (induction f)
-  case Nil
-  then show ?case by simp
-next
-  case Cons
-  fix f a
-  assume
-    prems: "findUnit (a # f) = Some x" and
-    IH: "findUnit f = Some x \<Longrightarrow> length (filter (notElem x) f) < length f"
-  then show "length (filter (notElem x) (a # f)) < length (a # f)"
-  proof (cases "notElem x a")
-    case
-      H1: True
-    then show ?thesis
-    proof (cases "findUnit f = Some x")
-      case True
-      with IH show ?thesis by simp
-    next
-      case False
-      then show ?thesis by (metis H1 One_nat_def Option.inject findUnit.simps(2) list.sel(1) list.size(3) n_not_Suc_n notElem.elims(2) prems)
-qed 
-next case False
-then show ?thesis by (simp add: filter.simps(2) le_imp_less_Suc length_Cons length_filter_le)
-qed
-qed
+(*second section of case has problem*)
+function  unitPropagate:: "Formula \<Rightarrow> Formula "
+where 
+"unitPropagate f = (case (findUnit f) of None \<Rightarrow>  f  | Some a \<Rightarrow> unitPropagate (resolve f a))"
+by pat_completeness auto
 
 
 lemma ter: "findUnit f = Some x \<Longrightarrow> length (filter (notElem x) f) < length f"
@@ -125,20 +86,21 @@ next
 qed
 
 
-(*second section of case has problem*)
-function  unitPropagate:: "Formula \<Rightarrow> Formula "
-where 
-"unitPropagate f = (case (findUnit f) of None \<Rightarrow>  f  | Some a \<Rightarrow> unitPropagate (resolve f a))"
-by pat_completeness auto
-
 termination 
 apply (relation "measure (\<lambda>x. size x)")
 apply (auto)
 apply (simp add: ter)
 done
 
-value "unitPropagate [[1,2],[1],[1,2]]"
-value "unitPropagate [[1,2,3]]"
+
+lemma [fundef_cong]:"(\<not>Q' \<Longrightarrow>  P=P') \<Longrightarrow> (Q=Q') \<Longrightarrow> (P \<or> Q)=(P'\<or> Q')"
+by blast
+
+function dpll:: "Formula \<Rightarrow> bool"
+where
+"dpll f = (if f = [] then True else if (elem [] f) then False else (let ff = unitPropagate f in(let nextLiteral = hd( hd f) in  dpll (resolve f (negateLiteral nextLiteral)) \<or>  dpll (resolve f nextLiteral))))"
+by pat_completeness auto 
+
 
 lemma ter2: "f \<noteq> [] \<Longrightarrow> \<not> elem [] f \<Longrightarrow> length (filter (notElem (hd (hd f))) f) < length f"
 proof (induction f)
@@ -176,19 +138,12 @@ then show ?thesis by (simp add: filter.simps(2) le_imp_less_Suc length_Cons leng
 qed
 qed
 
-lemma [fundef_cong]:"(\<not>Q' \<Longrightarrow>  P=P') \<Longrightarrow> (Q=Q') \<Longrightarrow> (P \<or> Q)=(P'\<or> Q')"
-by blast
-
-function dpll:: "Formula \<Rightarrow> bool"
-where
-"dpll f = (if f = [] then True else if (elem [] f) then False else (let ff = unitPropagate f in(let nextLiteral = hd( hd f) in  dpll (resolve f (negateLiteral nextLiteral)) \<or>  dpll (resolve f nextLiteral))))"
-by pat_completeness auto 
-
-
-
+lemma elim:"dpll_dom (map (removeAll (- hd (hd (a # f)))) (filter (notElem (hd (hd (a # f)))) (a # f))) \<Longrightarrow> length (filter (notElem (- hd (hd (a # f)))) (a # f)) < length (a # f)"
+apply (induction  rule: "dpll.pinduct") 
+sorry
 lemma ter3: "f \<noteq> [] \<Longrightarrow>
          \<not> elem [] f \<Longrightarrow>
-         \<not> dpll (map (removeAll (- hd (hd f))) (filter (notElem (hd (hd f))) f)) \<Longrightarrow>
+          \<not> dpll (map (removeAll (- hd (hd f))) (filter (notElem (hd (hd f))) f)) \<Longrightarrow>
          dpll_dom (map (removeAll (- hd (hd f))) (filter (notElem (hd (hd f))) f)) \<Longrightarrow>
          length (filter (notElem (- hd (hd f))) f) < length f"
 proof(induction f)
@@ -226,7 +181,7 @@ case True
 then show ?thesis
 proof (cases "dpll_dom (map (removeAll (- hd (hd (a#f)))) (filter (notElem (hd (hd (a#f)))) (a#f)))")
 case True
-then show ?thesis sorry 
+then show ?thesis using elim  by simp
 next 
 case False
 then show ?thesis using premssss by blast
@@ -247,9 +202,8 @@ then show ?thesis by (simp add: filter.simps(2) le_imp_less_Suc length_Cons leng
 qed
 qed
 
-
 termination
-apply (relation "measure (\<lambda>f. length f)")
+apply (relation "(measure (length))")
 apply auto
 apply (simp add:ter2)
 apply (simp add:ter3)
@@ -260,107 +214,33 @@ value "dpll [[-1]]"
 value "dpll []"
 
 
-lemma step_1:"f = [] \<Longrightarrow> dpll f = True"
-apply auto
-done 
-
-lemma step_2:"f \<noteq> [] \<Longrightarrow> elem [] f = True \<Longrightarrow> dpll f = False"
-apply auto
-done
-
-lemma step_3: "\<exists>m. dpll m = True"
-using step_1 by blast
-
-lemma step_4: "\<forall>f. f \<noteq> []  \<Longrightarrow>\<exists>m. dpll m = True"
-using step_3
-apply auto
-done
 (*============================================================================================*) 
-fun evalClause'::"Clause \<Rightarrow> Model \<Rightarrow> bool"
+fun validModel::"Model \<Rightarrow> bool"
 where
-"evalClause' [] m = False"
+"validModel [] = True"
 |
-"evalClause' (l#ls) m = (if l \<in> m then True else evalClause' ls m)"
+"validModel (m#rest) =(if m > 0 then True \<and> validModel rest else False  \<and> validModel rest)"
+
+
+fun evalLiteral::"Literal \<Rightarrow> Model \<Rightarrow> bool"
+where
+"evalLiteral l [] = (if l>0 then False else True)"
+|
+"evalLiteral l (m#ms) = (if (l > 0 ) \<and> (l = m) then True else if ((l < 0) \<and> ((-1*l) = m)) then False else evalLiteral l ms)"
+
+fun evalClause::"Clause \<Rightarrow> Model \<Rightarrow> bool"
+where
+"evalClause [] m = False"
+|
+"evalClause (l#ls) m = ((evalLiteral l m) \<or> evalClause ls m)"
 
 fun eval'::"Formula \<Rightarrow>Model \<Rightarrow>bool"
 where
 "eval' [] m = True"
 |
-"eval' (c#cs) m = ((evalClause' c m) \<and> (eval' cs m))"
+"eval' (c#cs) m = (((evalClause c m) \<and> (eval' cs m)))"
 
 
-
-lemma "\<forall>f. dpll f = True \<Longrightarrow>  \<exists>m. eval' f m =True"
-by (metis dpll.simps elem.simps(2) list.distinct(1))
-
-lemma "\<forall>f.  \<exists>m. eval' f m =True \<Longrightarrow> dpll f = True"
-using eval'.simps(2) evalClause'.simps(1) by blast
-
-lemma " (\<forall>f. dpll f = True) \<longleftrightarrow> (\<forall>f. \<exists>m. eval' f m =True)"
-by (metis elem.simps(2) eval'.simps(2) evalClause'.simps(1) list.distinct(1) step_2)
-
-
-lemma "(\<forall>f. dpll f = False \<Longrightarrow> \<forall>m. eval' f m = False)"
-using step_3 by auto
-
-lemma "\<forall>f m. eval' f m = False \<Longrightarrow>  dpll f = False"
-using eval'.simps(1) by auto
-
-lemma "(\<forall>f. dpll f = False) \<longleftrightarrow> (\<forall>f m. eval' f m = False)"
-using eval'.simps(1) step_1 by blast
-(*============================================================================================*)
-fun evalClause::"Formula \<Rightarrow> Literal \<Rightarrow> Formula"
-where
-"evalClause f l =  (resolve f l) "
-
-function eval::"Formula \<Rightarrow> Model \<Rightarrow> bool"
-where
-"eval f [] = (if f = [] then True else False)"
-|
-"eval f (m#ms)= (if f = [] then True else if elem [] f then False  else  eval (evalClause f m) ms)"
-apply auto
-by (meson list.exhaust)
-
-termination 
-
-apply (relation "measure (\<lambda>(f,m). length m)")
-apply auto
-done
-
-value"[[]] = []"
-
-
-lemma step_5[simp]:"eval [] [] = True"
-by simp
-
-lemma step_6[simp]:"f\<noteq>[] \<Longrightarrow> eval f [] = False"
-by simp
-
-lemma step_7[simp]:"eval [] m = True"
-using eval.elims(3) by fastforce
-
-value "dpll[[1,-1]]"
-
-lemma "\<forall>f. dpll f = True \<Longrightarrow>  \<exists>m. eval f m =True"
-using step_2 by fastforce
-
-lemma [simp]:"\<forall>f . \<exists>m. eval f m =True \<Longrightarrow> dpll f = True"
-apply (induction f)
-apply simp
-by (meson elem.simps(2) eval.elims(2) not_Cons_self2)
-
-
-lemma "(\<forall>f m. eval f m = False \<Longrightarrow>  dpll f = False)"
-apply (induction f)
-using step_5 apply auto[1]
-using step_5 by blast
-
-
-lemma [simp]:"(\<forall>f. dpll f = False \<Longrightarrow> \<forall>m. eval f m = False)"
-apply (induction f)
-apply simp
-apply metis
-using step_3 by blast
 
 end
 
