Isabelle/lemm.thy
@@ -1,0 +1,103 @@
+theory lemm 
+imports Main Simdpll
+begin
+lemma 1[simp]: "resolve [] a = []"
+apply simp
+done
+
+lemma yes: "findUnit f = Some x \<Longrightarrow> length (filter (notElem x) f) < length f"
+proof (induction f)
+  case Nil
+  then show ?case by simp
+next
+  case Cons
+  fix f a
+  assume
+    prems: "findUnit (a # f) = Some x" and
+    IH: "findUnit f = Some x \<Longrightarrow> length (filter (notElem x) f) < length f"
+  then show "length (filter (notElem x) (a # f)) < length (a # f)"
+  proof (cases "notElem x a")
+    case
+      H1: True
+    then show ?thesis
+    proof (cases "findUnit f = Some x")
+      case True
+      with IH show ?thesis by simp
+    next
+      case False
+      then show ?thesis by (metis H1 One_nat_def Option.inject findUnit.simps(2) list.sel(1) list.size(3) n_not_Suc_n notElem.elims(2) prems)
+qed 
+next case False
+then show ?thesis by (simp add: filter.simps(2) le_imp_less_Suc length_Cons length_filter_le)
+qed
+qed
+
+
+
+lemma ter: "findUnit f = Some x \<Longrightarrow> length (filter (notElem x) f) < length f"
+proof (induction f)
+  case Nil
+  then show ?case by simp
+next
+  case Cons
+  fix f a
+  assume
+    prems: "findUnit (a # f) = Some x" and
+    IH: "findUnit f = Some x \<Longrightarrow> length (filter (notElem x) f) < length f"
+  then show "length (filter (notElem x) (a # f)) < length (a # f)"
+  proof (cases "notElem x a")
+    case
+      H1: True
+    then show ?thesis
+    proof (cases "findUnit f = Some x")
+      case True
+      with IH show ?thesis by simp
+    next
+      case False
+      then have "Some (hd a) = Some x" "length a = 1"
+        using findUnit.simps prems by presburger+
+      then have "\<not> notElem x a" by (induction a) simp_all
+      with H1 show ?thesis by simp
+    qed
+  next
+    case False
+    then show ?thesis by (simp add: le_imp_less_Suc)
+  qed
+qed
+
+
+lemma step_1:"f = [] \<Longrightarrow> dpll f = True"
+apply auto
+done 
+
+lemma step_2:"f \<noteq> [] \<Longrightarrow> elem [] f = True \<Longrightarrow> dpll f = False"
+apply auto
+done
+
+lemma step_3: "\<exists>m. dpll m = True"
+using step_1 by blast
+
+lemma step_4: "\<forall>f. f \<noteq> []  \<Longrightarrow>\<exists>m. dpll m = True"
+using step_3
+apply auto
+done
+
+lemma "m = [] \<Longrightarrow> \<exists>f. validModel m  \<and> eval' f m =True"
+using eval'.simps(1) validModel.simps(1) by blast
+
+lemma st_1[simp]: "\<forall>f. dpll f = True \<Longrightarrow>  \<exists>m. validModel m  \<and> eval' f m =True"
+apply (induction f)
+using eval'.simps(1) validModel.simps(1) apply blast
+using step_2 by fastforce
+
+lemma st_2[simp]:"\<forall>f.  \<exists>m. validModel m  \<and>  eval' f m =True \<Longrightarrow> dpll f = True"
+using eval'.simps(2) evalClause.simps(1) by blast
+
+lemma st_3: "\<forall>f. dpll f = False \<Longrightarrow>  \<exists>m. validModel m =True  \<and> eval' f m =False"
+using st_1 
+using step_1 by blast
+
+lemma st_4[simp]:"\<forall>f. \<exists>m. validModel m =True  \<and> eval' f m =False \<Longrightarrow> dpll f = False"
+using st_2
+using eval'.simps(1) by blast
+end
